

(i) Given  $T(abc) = (2b+c, a-4b, 3a) *$

$$\text{Basis } = B' = \left\{ \underset{f_1}{(1, 1, 1)}, \underset{f_2}{(1, 1, 0)}, \underset{f_3}{(1, 0, 0)} \right\}$$

Step 1 Find  $T(f_1) = T(1, 1, 1)$   $T(f_2) = T(1, 1, 0)$

$T(f_3) = T(1, 0, 0)$  using \*

$$T(1, 1, 1) = \begin{pmatrix} 3 & -3 & 3 \end{pmatrix}$$

$$\text{iii) } T(1, 1, 0) = \begin{pmatrix} 2 & -3 & 3 \end{pmatrix}$$

$$T(1, 0, 0) = \begin{pmatrix} 0 & 1 & 3 \end{pmatrix}$$

in \*  
put  $(abc) = (1, 1, 1)$

Step 2 Express each of  $T(1, 1, 1)$   $T(1, 1, 0)$   $T(1, 0, 0)$  in terms of  $f_1$   $f_2$   $f_3$  as

$$\begin{aligned} x(1, 1, 1) + y(1, 1, 0) + z(1, 0, 0) &= (3, -3, 3) \\ &= (2, -3, 3) \\ &= (0, 1, 3) \end{aligned}$$

$$\Rightarrow \begin{array}{rcl} x + y + z = 3 & \text{OR} & 0 \\ x + y = -3 & & 0 \\ x = +3 & & 1 \end{array}$$

$$\text{1st} \quad \begin{array}{rcl} x + y + z = 3 & \text{Similar} & x + y + z = 0 \\ x + y = -3 & & x + y = 1 \\ x = +3 & & x = 3 \end{array}$$

$$\Rightarrow \begin{aligned} x &= +3 \\ y &= -6 \\ z &= 6 \end{aligned}$$

$$\Rightarrow \begin{aligned} x &= 3 \\ y &= -6 \\ z &= 5 \end{aligned}$$

$$\Rightarrow \begin{aligned} x &= 3 \\ y &= -2 \\ z &= -1 \end{aligned}$$

Matrix of LT with Basis B'

$$= [T]_{B'} = [A]_{B'} = \begin{bmatrix} 3 & -6 & 6 \\ 2 & -3 & 3 \\ 0 & 1 & 3 \end{bmatrix} = \begin{bmatrix} 3 & 3 & 2 \\ -6 & -6 & -2 \\ 6 & 5 & -1 \end{bmatrix}$$

Q Prove that  $T$  is invertible  
and find  $T^{-1}$  given

$$T(x_1, x_2, x_3) = (3x_1 + x_3, -2x_1 + x_2, -x_1 + 2x_2 + 4x_3) \quad (1)$$

Sol<sup>n</sup> wrt Std Base =  $\{(1\ 0\ 0), (0\ 1\ 0), (0\ 0\ 1)\}$

Matron of

$$\boxed{\phantom{000}} \quad (1)$$

$$\therefore A = \begin{bmatrix} 3 & 0 & 1 \\ -2 & 1 & 0 \\ -1 & 2 & 4 \end{bmatrix}$$

$$|A| = 9 \neq 0$$

$\Rightarrow A^{-1}$  exists

$\Rightarrow A$  is invertible

$\Rightarrow T$  is invertible

$$A^{-1} = \frac{1}{9} \begin{bmatrix} 4 & 2 & -1 \\ 8 & 13 & -2 \\ -3 & -6 & 3 \end{bmatrix}$$

$$\cancel{A^{-1}} A^{-1} \begin{bmatrix} x \\ y \\ z \end{bmatrix} = \frac{1}{9} \begin{bmatrix} 4 & 2 & -1 \\ 8 & 13 & -2 \\ -3 & -6 & 3 \end{bmatrix} \begin{bmatrix} x \\ y \\ z \end{bmatrix}$$

$$T^{-1}(x, y, z) = \left( \frac{4x + 2y - z}{9}, \frac{8x + 13y - 2z}{9}, \frac{-3x - 6y + 3z}{9} \right)$$

# Matrix of LT in different Basis

LinAlg  
Page 8  
Unit III

Q Find the matrix representation of the LT (OR Operator)  $T$  on  $\mathbb{R}^2$ .

(means  $T: \mathbb{R}^2 \rightarrow \mathbb{R}^2$ ) relative to standard or usual basis  $\{e_1, e_2\} \equiv \{(1,0), (0,1)\}$

$$\textcircled{1} T(x, y) = (2y, 3x - y)$$

$$\textcircled{2} T(x, y) = (3x - 4y, x + 5y)$$

Soln  $\textcircled{1}$  Give  $T: \mathbb{R}^2 \rightarrow \mathbb{R}^2$ ,  $T(x, y) = (2y, 3x - y)$   
 $= (0x + 2y, 3x - y)$

Matrix of LT  $T$  is  $A = \begin{bmatrix} 0 & 2 \\ 3 & -1 \end{bmatrix}$

---

$$\textcircled{2} T(x, y) = (3x - 4y, x + 5y) \quad A = \begin{bmatrix} 3 & -4 \\ 1 & 5 \end{bmatrix}$$

Q Find the matrix representation of LT ~~on~~ given previous example (page 8) wrt basis

$$\{f_1, f_2\} = \{(1, 3), (2, 5)\}$$

Soln Given Two L.T.  $T: \mathbb{R}^2 \rightarrow \mathbb{R}^2$

$$(i) T(x, y) = (2y, 3x-y)$$

$$(ii) T(x, y) = (3x-4y, x+5y)$$

Basis  $\{f_1, f_2\} = \{(1, 3), (2, 5)\} = B$  (say)

(i) Consider  $T(x, y) = (2y, 3x-y)$  ①  
To find matrix of  $T$  wrt Basis  $\{f_1, f_2\} = B$

Step 1  $\Rightarrow$  In ① find  $T(1, 3)$   $T(2, 5)$

$$T(1, 3) = (6, 0)$$

$$T(2, 5) = (10, 1)$$

Step 2 Express  $T(1, 3)$  &  $T(2, 5)$  in terms of  $f_1, f_2$

②  $\begin{aligned} T(f_1) &= (6, 0) = x f_1 + y f_2 \\ T(f_2) &= (10, 1) = x f_1 + y f_2 \end{aligned}$

$$\Rightarrow \begin{aligned} (6, 0) &= x(1, 3) + y(2, 5) \\ (10, 1) &= x(1, 3) + y(2, 5) \end{aligned}$$

$$\begin{cases} x+2y = 6 \\ 3x+5y = 0 \end{cases}$$

$$\begin{cases} x+2y = 10 \\ 3x+5y = 1 \end{cases}$$

$$S = \left[ \begin{array}{cc|cc} 1 & 2 & 6 & 10 \\ 3 & 5 & 0 & 1 \end{array} \right]$$

$$\begin{array}{l} R_2 - 3R_1 \\ \sim \end{array} \left[ \begin{array}{cc|cc} 1 & 2 & 6 & 10 \\ 0 & -1 & -18 & -29 \end{array} \right]$$

$$\left\{ \begin{array}{l} x + 2y = 6 \\ -y = -18 \end{array} \right. \text{ and } \left\{ \begin{array}{l} x + 2y = 10 \\ -y = -29 \end{array} \right.$$

OR

$$\left\{ \begin{array}{l} y = 18 \\ x = -30 \end{array} \right. \quad \left\{ \begin{array}{l} y = 29 \\ x = -48 \end{array} \right.$$

Put them in ②

$$\begin{aligned} T(f_1) &= T(1, 3) = (6, 0) = -30f_1 + 18f_2 \\ T(f_2) &= T(2, 5) = (10, 1) = -48f_1 + 29f_2 \end{aligned}$$

\* Matrix of  $[T]_f = \begin{pmatrix} -30 & -48 \\ 18 & 29 \end{pmatrix}$

Similarly, For  $T(x, y) = (3x - 4y, x + 5y)$

(ii)

$$A = \begin{pmatrix} 3 & -4 \\ 1 & 5 \end{pmatrix}$$